Basic Checker Setup

Auto/Embedding/LamBase.lean
@@ -924,7 +924,7 @@ def LamTerm.lamCheck!_of_lamWF {default : LamSort}
 -- This function is meant to be `execute`-d (`eval`-ed), not `reduce`-d
 -- **TODO**: Change type to `match` so that we don't need `rw`.
 --   But do not delete this, because it shows problems (proof not fully reducing)
-def LamWF.ofCheck? {ltv : LamTyVal} :
+def LamWF.ofLamCheck? {ltv : LamTyVal} :
   {lctx : Nat → LamSort} → {t : LamTerm} → {ty : LamSort} →
   t.lamCheck? ltv lctx = .some ty → LamWF ltv ⟨lctx, t, ty⟩
 | lctx, .atom n, ty, HCheck => by
@@ -940,7 +940,7 @@ def LamWF.ofCheck? {ltv : LamTyVal} :
   case none => intro contra; cases contra
   case some bodyTy =>
     dsimp; intro tyEq; rw [← Option.some.inj tyEq]
-    apply LamWF.ofLam; apply (ofCheck? CheckEq)
+    apply LamWF.ofLam; apply (ofLamCheck? CheckEq)
 | lctx, .app s fn arg, ty, HCheck => by
   simp [LamTerm.lamCheck?] at HCheck; revert HCheck
   match CheckFnEq : LamTerm.lamCheck? ltv lctx fn, CheckArgEq : LamTerm.lamCheck? ltv lctx arg with
@@ -955,22 +955,22 @@ def LamWF.ofCheck? {ltv : LamTyVal} :
     case true =>
       dsimp;
       intro H; rw [← Option.some.inj H]; apply LamWF.ofApp (argTy:=s);
-      case HFn => apply (ofCheck? CheckFnEq)
-      case HArg => apply (ofCheck? CheckArgEq)
+      case HFn => apply (ofLamCheck? CheckFnEq)
+      case HArg => apply (ofLamCheck? CheckArgEq)
   | .some (LamSort.func _ _), .none => intro contra; cases contra
   | .some (LamSort.atom _), _ => intro contra; cases contra
   | .some (LamSort.base _), _ => intro contra; cases contra
   | .none, _ => intro contra; cases contra
 
 /-
-#reduce @LamWF.ofCheck?
+#reduce @LamWF.ofLamCheck?
   (ltv := {(Inhabited.default : LamTyVal) with lamVarTy := fun n => .atom 0})
   (lctx := fun _ => .atom 0)
   (t := .atom 0)
   (ty := .atom 0)
   rfl
 
-#reduce @LamWF.ofCheck?
+#reduce @LamWF.ofLamCheck?
   (ltv := {(Inhabited.default : LamTyVal) with
     lamVarTy := fun n => if n == 0 then .func (.atom 0) (.atom 0) else .atom 0})
   (lctx := fun _ => .atom 0)
@@ -978,7 +978,7 @@ def LamWF.ofCheck? {ltv : LamTyVal} :
   (ty := .atom 0)
   rfl
 
-#reduce @LamWF.ofCheck?
+#reduce @LamWF.ofLamCheck?
   (ltv := {(Inhabited.default : LamTyVal) with
     lamVarTy := fun n => if n == 0 then .atom 2 else .func (.atom 2) (.atom 1)})
   (lctx := fun _ => .atom 0)
@@ -986,7 +986,7 @@ def LamWF.ofCheck? {ltv : LamTyVal} :
   (ty := .func (.atom 0) (.atom 1))
   rfl
 
-#eval @LamWF.ofCheck?
+#eval @LamWF.ofLamCheck?
   (ltv := {(Inhabited.default : LamTyVal) with
     lamVarTy := fun n => if n == 0 then .atom 2 else .func (.atom 2) (.atom 1)})
   (lctx := fun _ => .atom 0)
@@ -1636,7 +1636,7 @@ def LamThmWF
   (lval : LamValuation) (lctx : List LamSort) (rty : LamSort) (t : LamTerm) :=
   ∀ (lctx' : Nat → LamSort), LamWF lval.ilVal.toLamTyVal ⟨pushLCtxs lctx lctx', t, rty⟩
 
-def LamThmWF' (lval : LamValuation) (lctx : List LamSort) (rty : LamSort) (t : LamTerm) :=
+def LamThmWFP (lval : LamValuation) (lctx : List LamSort) (rty : LamSort) (t : LamTerm) :=
   ∀ (lctx' : Nat → LamSort), Nonempty (LamWF lval.ilVal.toLamTyVal ⟨pushLCtxs lctx lctx', t, rty⟩)
 
 def LamThmValid (lval : LamValuation) (lctx : List LamSort) (t : LamTerm) :=
@@ -1650,6 +1650,28 @@ def LamThmValid (lval : LamValuation) (lctx : List LamSort) (t : LamTerm) :=
 @[reducible] def dfLCtxTerm (val : Nat → Type u) : ∀ n, LamSort.interp val (dfLCtxTy n) :=
   fun _ => GLift.up.{1, u} False
 
+theorem LamThmWFP.ofLamThmWF (H : LamThmWF lval lctx s t) :
+  LamThmWFP lval lctx s t :=
+  fun lctx => Nonempty.intro (H lctx)
+
+theorem LamThmWF.ofLamThmWFP (H : LamThmWFP lval lctx s t) :
+  LamThmWF lval lctx s t := by
+  intro lctx'; cases h₁ : LamTerm.lamCheck? lval.ilVal.toLamTyVal (pushLCtxs lctx lctx') t
+  case none =>
+    apply False.elim; have ⟨wf⟩ := H lctx'
+    have hChk := LamTerm.lamCheck?_of_lamWF wf
+    rw [h₁] at hChk; cases hChk
+  case some s' =>
+    cases h₂ : s'.beq s
+    case false =>
+      apply False.elim; have ⟨wf⟩ := H lctx'
+      have hChk := LamTerm.lamCheck?_of_lamWF wf
+      rw [h₁] at hChk; rw [Option.some.inj hChk] at h₂
+      rw [LamSort.beq_refl] at h₂; cases h₂
+    case true =>
+      rw [LamSort.beq_eq _ _ h₂] at h₁
+      apply LamWF.ofLamCheck? h₁
+
 def LamThmWF.append (H : LamThmWF lval lctx rty t) (ex : List LamSort) :
   LamThmWF lval (lctx ++ ex) rty t := by
   dsimp [LamThmWF]; intros lctx'; rw [pushLCtxs.append]; apply H
@@ -1660,11 +1682,11 @@ def LamThmWF.prepend (H : LamThmWF lval lctx rty t) (ex : List LamSort) :
   rw [pushLCtxs.append]; rw [← pushLCtxsAt.zero ex]
   apply LamWF.ofBVarLiftsIdx (idx:=0); rfl; apply H
 
-theorem LamThmWF.ofCheck?
+theorem LamThmWF.ofLamCheck?
   {lval : LamValuation} {lctx : List LamSort} {rty : LamSort} {t : LamTerm}
   (h₁ : LamTerm.lamCheck? lval.ilVal.toLamTyVal (pushLCtxs lctx dfLCtxTy) t = .some rty)
   (h₂ : t.maxLooseBVarSucc ≤ lctx.length) : LamThmWF lval lctx rty t := by
-  intros lctx'; apply LamWF.ofCheck?; apply Eq.trans _ h₁
+  intros lctx'; apply LamWF.ofLamCheck?; apply Eq.trans _ h₁
   apply LamTerm.lamCheck?_irrelevence; intro n hlt; dsimp [pushLCtxs]
   have hlt' : n < List.length lctx := Nat.le_trans hlt h₂
   have htrue : Nat.blt n (List.length lctx) = true := by
@@ -1672,15 +1694,9 @@ theorem LamThmWF.ofCheck?
   rw [htrue]; dsimp;
   rw [List.getD_eq_get _ _ hlt']; rw [List.getD_eq_get _ _ hlt']
 
-theorem LamThmWF'.ofLamThmValid (H : LamThmValid lval lctx t) :
-  LamThmWF' lval lctx (.base .prop) t :=
-  fun lctx => let ⟨wf, _⟩ := H lctx; Nonempty.intro wf
-
-theorem LamThmWF'.ofCheck?
-  {lval : LamValuation} {lctx : List LamSort} {rty : LamSort} {t : LamTerm}
-  (h₁ : LamTerm.lamCheck? lval.ilVal.toLamTyVal (pushLCtxs lctx dfLCtxTy) t = .some rty)
-  (h₂ : t.maxLooseBVarSucc ≤ lctx.length) : LamThmWF' lval lctx rty t := by
-  intro lctx'; apply Nonempty.intro; apply LamThmWF.ofCheck? h₁ h₂
+theorem LamThmWF.ofLamThmValid (H : LamThmValid lval lctx t) :
+  LamThmWF lval lctx (.base .prop) t :=
+  LamThmWF.ofLamThmWFP (fun lctx => let ⟨wf, _⟩ := H lctx; Nonempty.intro wf)
 
 theorem LamThmValid.append (H : LamThmValid lval lctx t)
   (ex : List LamSort) : LamThmValid lval (lctx ++ ex) t := by
@@ -1739,7 +1755,7 @@ theorem LamThmValid.ofInterpAsProp
   intros lctx';
   have h₁' := Eq.trans (LamTerm.lamCheck?_irrelevence (lctx₁:=lctx') (by
     intro n hlt; rw [h₃] at hlt; cases hlt)) h₁
-  have wf := LamWF.ofCheck? h₁'; exists wf; intros lctxTerm
+  have wf := LamWF.ofLamCheck? h₁'; exists wf; intros lctxTerm
   apply Eq.mp _ h₂
   apply congrArg; apply eq_of_heq;
   apply HEq.trans (LamTerm.interpAsProp.equiv _ _ _ _ (LamTerm.lamCheck.equiv _ h₁))
@@ -1747,7 +1763,7 @@ theorem LamThmValid.ofInterpAsProp
     apply HEq.trans _ (LamWF.interp_irrelevance
       (lctxTy₁:=dfLCtxTy) (lctxTerm₁:=dfLCtxTerm _) _ _ _)
     case _ =>
-      apply LamThmWF.ofCheck? (lctx:=[]) _ _ dfLCtxTy
+      apply LamThmWF.ofLamCheck? (lctx:=[]) _ _ dfLCtxTy
       rw [pushLCtxs.nil, h₁]
       rw [h₃]; exact .refl
     case _ => apply HEq.symm; apply LamTerm.interp.equiv
